model/structures/StepQsec.v
@@ -1,0 +1,321 @@
+Require Export QArith.
+Require Export StepFunctionSetoid.
+Require Import Qabs.
+Require Import Bool.
+Require Import CornTac.
+
+Set Implicit Arguments.
+
+Open Local Scope sfstscope.
+
+Section QS.
+
+Lemma QS:(Setoid).
+exists Q Qeq.
+split; eauto with qarith.
+Defined.
+
+Definition QabsS : QS-->QS.
+exists Qabs.
+abstract(
+simpl; intros x1 x2 Hx;
+rewrite Hx;
+reflexivity).
+Defined.
+
+Definition Qplus0 : QS -> QS --> QS.
+intros q.
+exists (Qplus q).
+abstract (
+simpl; intros x1 x2 Hx;
+rewrite Hx;
+reflexivity).
+Defined.
+
+Definition QplusS : QS --> QS --> QS.
+exists (Qplus0).
+abstract (
+intros x1 x2 Hx y; simpl in *;
+rewrite Hx;
+reflexivity).
+Defined.
+
+Definition QoppS : QS --> QS.
+exists (Qopp).
+abstract (
+simpl; intros x1 x2 Hx; simpl in *;
+rewrite Hx;
+reflexivity).
+Defined.
+
+Definition Qminus0 : QS -> QS --> QS.
+intros q.
+exists (Qminus q).
+abstract (
+simpl; intros x1 x2 Hx;
+rewrite Hx;
+reflexivity).
+Defined.
+
+Definition QminusS : QS --> QS --> QS.
+exists (Qminus0).
+abstract (
+intros x1 x2 Hx y; simpl in *;
+rewrite Hx;
+reflexivity).
+Defined.
+
+Definition QscaleS : QS -> QS --> QS.
+intros q.
+exists (Qmult q).
+abstract (
+intros x1 x2 Hx; simpl in *;
+rewrite Hx;
+reflexivity).
+Defined.
+
+Definition QmultS : QS --> QS --> QS.
+exists (QscaleS).
+abstract (
+intros x1 x2 Hx y; simpl in *;
+rewrite Hx;
+reflexivity).
+Defined.
+
+Definition Qle0 : QS -> QS --> iffSetoid.
+intros q.
+exists (Qle q).
+abstract (
+simpl; intros x1 x2 Hx;
+rewrite Hx;
+reflexivity).
+Defined.
+
+Definition QleS : QS --> QS --> iffSetoid.
+exists (Qle0).
+abstract (
+intros x1 x2 Hx y; simpl in *;
+rewrite Hx;
+reflexivity).
+Defined.
+
+End QS.
+
+Definition StepQ := (StepF QS).
+
+Definition StepQplus (s t:StepQ) : StepQ := QplusS ^@> s <@> t.
+Definition StepQopp (s:StepQ) : StepQ := QoppS ^@> s.
+Definition StepQminus (s t:StepQ) : StepQ := QminusS ^@> s <@> t.
+Definition StepQmult (s t:StepQ) : StepQ := QmultS ^@> s <@> t.
+Notation "x + y" := (StepQplus x y) : StepQ_scope.
+Notation "- x" := (StepQopp x) : StepQ_scope.
+Notation "x - y" := (StepQminus x y) : StepQ_scope.
+Notation "x * y" := (StepQmult x y) : StepQ_scope.
+
+Delimit Scope StepQ_scope with StepQ.
+Bind Scope StepQ_scope with StepQ.
+
+Open Local Scope StepQ_scope.
+
+Add Morphism StepQplus with signature StepF_eq ==> StepF_eq ==> StepF_eq as StepQplus_wd.
+Proof.
+intros.
+unfold StepQplus.
+rewrite H.
+rewrite H0.
+reflexivity.
+Qed.
+
+Add Morphism StepQopp with signature StepF_eq ==> StepF_eq as StepQopp_wd.
+Proof.
+intros.
+unfold StepQopp.
+rewrite H.
+reflexivity.
+Qed.
+
+Add Morphism StepQminus with signature StepF_eq ==> StepF_eq ==> StepF_eq as StepQminus_wd.
+Proof.
+intros.
+unfold StepQminus.
+rewrite H.
+rewrite H0.
+reflexivity.
+Qed.
+
+Add Morphism StepQmult with signature StepF_eq ==> StepF_eq ==> StepF_eq as StepQmult_wd.
+Proof.
+intros.
+unfold StepQmult.
+rewrite H.
+rewrite H0.
+reflexivity.
+Qed.
+
+Definition StepQsrt : (@ring_theory (StepQ) (constStepF (0:QS)) (constStepF (1:QS)) StepQplus StepQmult StepQminus StepQopp (@StepF_eq QS)).
+constructor; 
+ intros; 
+ unfold StepF_eq, StepQplus, StepQminus, StepQopp, StepQmult; 
+ rewriteStepF;
+ set (g:=st_eqS QS).
+
+set (z:=QplusS 0).
+set (f:=(join (compose g z))).
+cut (StepFfoldProp (f ^@> x)).
+ unfold f; evalStepF; tauto.
+apply StepFfoldPropForall_Map.
+intros a.
+unfold f; simpl; ring.
+
+set (f:=ap
+ (compose (@ap _ _ _) (compose (compose g) QplusS))
+ (flip (QplusS))).
+cut (StepFfoldProp (f ^@> x <@> y)).
+ unfold f; evalStepF; tauto.
+apply StepFfoldPropForall_Map2.
+intros a b.
+change (a + b == b + a)%Q.
+ring.
+
+set (f:=ap
+ (compose (@ap _ _ _) (compose (compose (compose (compose (@ap _ _ _)) (@compose _ _ _) g)) (compose (flip (@compose _ _ _) QplusS) (compose (@compose _ _ _) QplusS))))
+ (compose (compose QplusS) QplusS)).
+cut (StepFfoldProp (f ^@> x <@> y <@> z)).
+ unfold f; evalStepF; tauto.
+apply StepFfoldPropForall_Map3.
+intros a b c.
+change (a + (b + c) == a + b + c)%Q.
+ring.
+
+set (z:=(QmultS 1)).
+set (f:=(join (compose g z))).
+cut (StepFfoldProp (f ^@> x)).
+ unfold f; evalStepF; tauto.
+apply StepFfoldPropForall_Map.
+intros a.
+unfold f; simpl; ring.
+
+set (f:=ap
+ (compose (@ap _ _ _) (compose (compose g) QmultS))
+ (flip (QmultS))).
+cut (StepFfoldProp (f ^@> x <@> y)).
+ unfold f; evalStepF; tauto.
+apply StepFfoldPropForall_Map2.
+intros a b.
+change (a * b == b * a)%Q.
+ring.
+
+set (f:=ap
+ (compose (@ap _ _ _) (compose (compose (compose (compose (@ap _ _ _)) (@compose _ _ _) g)) (compose (flip (@compose _ _ _) QmultS) (compose (@compose _ _ _) QmultS))))
+ (compose (compose QmultS) QmultS)).
+cut (StepFfoldProp (f ^@> x <@> y <@> z)).
+ unfold f; evalStepF; tauto.
+apply StepFfoldPropForall_Map3.
+intros a b c.
+change (a * (b * c) == a * b * c)%Q.
+ring.
+
+set (f:= ap
+ (compose (@ap _ _ _) (compose (compose (compose (@ap _ _ _) (compose (compose g) QmultS))) QplusS))
+ (compose (flip (@compose _ _ _) QmultS) (compose (@ap _ _ _) (compose (compose QplusS) QmultS)))).
+cut (StepFfoldProp (f ^@> x <@> y <@> z)).
+ unfold f; evalStepF; tauto.
+apply StepFfoldPropForall_Map3.
+intros a b c.
+change ((a + b) * c == a*c + b*c)%Q.
+ring.
+
+set (f:= ap
+ (compose (@ap _ _ _) (compose (compose g) QminusS))
+ (compose (flip (@compose _ _ _) QoppS) QplusS)).
+cut (StepFfoldProp (f ^@> x <@> y)).
+ unfold f; evalStepF; tauto.
+apply StepFfoldPropForall_Map2.
+intros a b.
+change (a - b == a + - b)%Q.
+ring.
+
+set (z:=(0:QS)).
+set (f:= compose (flip g z) (ap QplusS QoppS)).
+cut (StepFfoldProp (f ^@> x)).
+ unfold f; evalStepF; tauto.
+apply StepFfoldPropForall_Map.
+intros a.
+change (a + - a == 0)%Q.
+ring.
+Qed.
+
+Definition StepQisZero:(StepQ)->bool:=(StepFfold (fun (x:QS) => Qeq_bool x 0) (fun _  x y => x && y)).
+
+Definition StepQeq_bool (x y:StepQ) : bool := StepQisZero (x-y).
+
+Lemma StepQeq_bool_correct : forall x y, StepQeq_bool x y = true -> x == y.
+Proof.
+intros x y H.
+destruct StepQsrt.
+rewrite <- (Radd_0_l x).
+rewrite <- (Ropp_def y).
+transitivity (y + (constStepF (0:QS))).
+ set (z:=constStepF (X:=QS) 0).
+ rewrite <- (Radd_assoc).
+ apply StepQplus_wd.
+  reflexivity.
+ rewrite Radd_comm.
+ rewrite <- Rsub_def.
+ unfold StepF_eq.
+ revert H.
+ unfold StepQeq_bool.
+ generalize (x-y).
+ intros s H.
+ induction s.
+  rapply Qeq_bool_correct.
+  assumption.
+ symmetry in H.
+ destruct (andb_true_eq _ _ H) as [H1 H2].
+ split.
+  apply IHs1; symmetry; assumption.
+ apply IHs2; symmetry; assumption.
+rewrite Radd_comm.
+apply Radd_0_l.
+Qed.
+
+Lemma StepQRing_Morphism : ring_eq_ext StepQplus StepQmult StepQopp (@StepF_eq QS).
+split.
+  apply StepQplus_wd.
+ apply StepQmult_wd.
+apply StepQopp_wd.
+Qed.
+
+Ltac isStepQcst t :=
+  match t with
+  | constStepF ?q => isQcst q
+  | glue ?o ?l ?r => 
+   match isStepQcst l with
+   |true => match isStepQcst r with
+            |true => isQcst o
+            |false => false
+            end
+   |false => false
+   end
+  end.
+
+Ltac StepQcst t :=
+  match isStepQcst t with
+    true => t
+    | _ => NotConstant
+  end.
+
+Add Ring StepQRing : StepQsrt
+ (decidable StepQeq_bool_correct,
+  setoid (StepF_Sth QS) StepQRing_Morphism,
+  constants [StepQcst]).
+
+Definition StepQabs (s:StepQ) : StepQ := QabsS ^@> s.
+
+Add Morphism StepQabs with signature StepF_eq ==> StepF_eq as StepQabs_wd.
+Proof.
+intros.
+unfold StepQabs.
+rewrite H.
+reflexivity.
+Qed.
